typ: style and reorg

src/typ/core.lean
@@ -1,78 +1,25 @@
-import data.finset
-import data.fresh
-import data.list.extra
-import occurs
+import data.fresh occurs
 
 namespace tts ------------------------------------------------------------------
 
--- Grammar of types.
+/-- Grammar of types -/
 @[derive decidable_eq]
 inductive typ (V : Type) : Type
-  | var : occurs → tagged V → typ -- variable, bound or free
-  | arr : typ → typ → typ         -- function arrow
-
-variables {V : Type} -- Type of variable names
+| var : occurs → tagged V → typ -- variable, bound or free
+| arr : typ → typ → typ         -- function arrow
 
 namespace typ ------------------------------------------------------------------
-variables [_root_.decidable_eq V]
+variables {V : Type} -- Type of variable names
 
 open occurs
 
-protected
-def repr [has_repr V] : typ V → string
-  | (var bound x)  := _root_.repr x.tag ++ "⟨" ++ _root_.repr x.val ++ "⟩"
-  | (var free x)   := _root_.repr x
-  | (arr t₁ t₂)    := "(" ++ t₁.repr ++ ") → (" ++ t₂.repr ++ ")"
+protected def repr [has_repr V] : typ V → string
+| (var bound x)  := _root_.repr x.tag ++ "⟨" ++ _root_.repr x.val ++ "⟩"
+| (var free x)   := _root_.repr x
+| (arr t₁ t₂)    := "(" ++ t₁.repr ++ ") → (" ++ t₂.repr ++ ")"
 
 instance [has_repr V] : has_repr (typ V) :=
 ⟨typ.repr⟩
-
--- Free variables of a type
-def fv : typ V → finset (tagged V)
-  | (var bound _) := ∅
-  | (var free x)  := {x}
-  | (arr t₁ t₂)   := fv t₁ ∪ fv t₂
-
--- Free variables of a list of types
-def fv_list : list (typ V) → finset (tagged V)
-  | []        := ∅
-  | (t :: ts) := fv t ∪ fv_list ts
-
--- Substitute a free variable for a type in a type
-def subst (x : tagged V) (t : typ V) : typ V → typ V
-  | (var bound y)  := var bound y
-  | (var free y)   := if x = y then t else var free y
-  | (arr t₁ t₂)    := arr (subst t₁) (subst t₂)
-
--- Substitute a list of free variables for a list of types in a type
-def subst_list : list (tagged V) → list (typ V) → typ V → typ V
-  | (x :: xs) (t₂ :: ts₂) t₁ := subst_list xs ts₂ (subst x t₂ t₁)
-  | _         _           t₁ := t₁
-
--- Open a type with a list of types for bound variables.
-@[simp]
-def open_typs (ts : list (typ V)) : typ V → typ V
-  | (var bound x) := (ts.nth x.tag).get_or_else (var bound x)
-  | (var free x)  := var free x
-  | (arr t₁ t₂)   := arr (open_typs t₁) (open_typs t₂)
-
--- Open a type with a list of free variables for bound variables.
-def open_vars (xs : list (tagged V)) (t : typ V) : typ V :=
-  open_typs (list.map (var free) xs) t
-
--- Property of a locally-closed type.
-inductive lc : typ V → Prop
-  | var : Π (x : tagged V),                  lc (var free x)
-  | arr : Π {t₁ t₂ : typ V}, lc t₁ → lc t₂ → lc (arr t₁ t₂)
-
--- Locally-closed body of a type scheme with a given arity
-def lc_body (n : ℕ) (t : typ V) : Prop :=
-  ∃ (L : finset (tagged V)),
-  ∀ {xs : list (tagged V)},
-  xs.nodup →
-  xs.length = n →
-  (∀ {x : tagged V}, x ∈ xs → x ∉ L) →
-  lc (open_vars xs t)
 
 end /- namespace -/ typ --------------------------------------------------------
 end /- namespace -/ tts --------------------------------------------------------
