src/typ/fv.lean
@@ -2,34 +2,38 @@ import .core
 
 namespace tts ------------------------------------------------------------------
 namespace typ ------------------------------------------------------------------
-variables {V : Type} -- Type of variable names
-variables {x x₁ x₂ : tagged V} -- Variable
+variables {V : Type} [_root_.decidable_eq V] -- Type of variable names
+variables {x y : tagged V} -- Variable
 variables {t t₁ t₂ : typ V} -- Types
 variables {ts ts₁ ts₂ : list (typ V)} -- Lists of types
 
-variables [_root_.decidable_eq V]
-
 open occurs
 
-@[simp]
-theorem fv_not_mem_var_free : x₁ ∉ fv (var free x₂) ↔ x₁ ≠ x₂ :=
-  by simp [fv]
+/-- Free variables of a type -/
+def fv : typ V → finset (tagged V)
+| (var bound _) := ∅
+| (var free x)  := {x}
+| (arr t₁ t₂)   := fv t₁ ∪ fv t₂
 
-@[simp]
-theorem fv_not_mem_arr : x ∉ fv (arr t₁ t₂) ↔ x ∉ fv t₁ ∧ x ∉ fv t₂ :=
-  by simp [fv, decidable.not_or_iff_and_not]
+@[simp] theorem fv_not_mem_var_free : x ∉ fv (var free y) ↔ x ≠ y :=
+by simp [fv]
 
-@[simp]
-theorem fv_list_nil : fv_list ([] : list (typ V)) = ∅ :=
-  rfl
+@[simp] theorem fv_not_mem_arr : x ∉ fv (arr t₁ t₂) ↔ x ∉ fv t₁ ∧ x ∉ fv t₂ :=
+by simp [fv, not_or_distrib]
 
-@[simp]
-theorem fv_list_cons : fv_list (t :: ts) = fv t ∪ fv_list ts :=
-  rfl
+/-- Free variables of a list of types -/
+def fv_list : list (typ V) → finset (tagged V)
+| []        := ∅
+| (t :: ts) := fv t ∪ fv_list ts
 
-@[simp]
-theorem fv_list_append : fv_list (ts₁ ++ ts₂) = fv_list ts₁ ∪ fv_list ts₂ :=
-  by induction ts₁ with _ _ ih; [simp, simp [ih]]
+@[simp] theorem fv_list_nil : fv_list ([] : list (typ V)) = ∅ :=
+rfl
+
+@[simp] theorem fv_list_cons : fv_list (t :: ts) = fv t ∪ fv_list ts :=
+rfl
+
+@[simp] theorem fv_list_append : fv_list (ts₁ ++ ts₂) = fv_list ts₁ ∪ fv_list ts₂ :=
+by induction ts₁ with _ _ ih; [simp, simp [ih]]
 
 end /- namespace -/ typ --------------------------------------------------------
 end /- namespace -/ tts --------------------------------------------------------
