src/typ/lc.lean
@@ -1,23 +1,36 @@
-import .core
+import typ.open
 
 namespace tts ------------------------------------------------------------------
 namespace typ ------------------------------------------------------------------
-variables {V : Type} -- Type of variable names
-variables {t₁ t₂ : typ V} -- Types
-
-variables [_root_.decidable_eq V]
+variables {V : Type} [_root_.decidable_eq V] -- Type of variable names
+variables {t t₁ t₂ : typ V} -- Types
+variables {ts : list (typ V)} -- Lists of types
 
 open occurs
 
-@[simp]
-theorem lc_var_free (x : tagged V) : lc (var free x) :=
-  lc.var x
+/-- Locally-closed type -/
+inductive lc : typ V → Prop
+| var : Π (x : tagged V),                  lc (var free x)
+| arr : Π {t₁ t₂ : typ V}, lc t₁ → lc t₂ → lc (arr t₁ t₂)
 
-@[simp]
-theorem lc_arr : lc (arr t₁ t₂) ↔ lc t₁ ∧ lc t₂ :=
-  ⟨ λ l, by cases l with _ _ _ l₁ l₂; exact ⟨l₁, l₂⟩
-  , λ ⟨l₁, l₂⟩, lc.arr l₁ l₂
-  ⟩
+/-- Locally-closed body of a type scheme with a given arity -/
+def lc_body (n : ℕ) (t : typ V) : Prop :=
+∃ (L : finset (tagged V)),
+∀ {xs : list (tagged V)},
+xs.nodup →
+xs.length = n →
+(∀ {x : tagged V}, x ∈ xs → x ∉ L) →
+lc (open_vars xs t)
+
+@[simp] theorem lc_var_free (x : tagged V) : lc (var free x) :=
+lc.var x
+
+@[simp] theorem lc_arr : lc (arr t₁ t₂) ↔ lc t₁ ∧ lc t₂ :=
+⟨λ l, by cases l with _ _ _ l₁ l₂; exact ⟨l₁, l₂⟩, λ ⟨l₁, l₂⟩, lc.arr l₁ l₂⟩
+
+-- Opening a locally-closed type is the identity
+@[simp] theorem open_typs_id (l : lc t) : open_typs ts t = t :=
+by induction t; cases l; simp [open_typs, *]
 
 end /- namespace -/ typ --------------------------------------------------------
 end /- namespace -/ tts --------------------------------------------------------
