src/typ/subst.lean
@@ -1,198 +1,179 @@
-import .fv
-import .lc
-import typ.open
-import data.finset
-import logic.extra
+import data.list.extra .fv .lc
 
 local attribute [simp] not_or_distrib and_assoc
 
-
 namespace tts ------------------------------------------------------------------
 namespace typ ------------------------------------------------------------------
-variables {V : Type} -- Type of variable names
+variables {V : Type} [_root_.decidable_eq V] -- Type of variable names
 variables {x y : tagged V} -- Variables
-variables {xs : list (tagged V)} -- List of variable names
+variables {xs : list (tagged V)} -- List of variables
 variables {t tx t₁ t₂ : typ V} -- Types
-variables {ts ts₁ ts₂ : list (typ V)} -- Lists of types
+variables {ts txs ts₂ : list (typ V)} -- Lists of types
 
-variables [_root_.decidable_eq V]
+open list occurs
 
-open occurs
+/- subst -/
 
-@[simp]
-theorem subst_var_bound : subst x t (var bound y) = var bound y :=
-  rfl
+/-- Substitute a free variable for a type in a type -/
+def subst (x : tagged V) (tx : typ V) : typ V → typ V
+| (var bound y)  := var bound y
+| (var free y)   := if x = y then tx else var free y
+| (arr t₁ t₂)    := arr (subst t₁) (subst t₂)
 
-@[simp]
-theorem subst_var_free_eq (h : x = y) : subst x t (var free y) = t :=
-  by simp [subst, h]
+@[simp] theorem subst_var_bound : subst x tx (var bound y) = var bound y :=
+rfl
 
-@[simp]
-theorem subst_var_free_ne (h : x ≠ y) : subst x t (var free y) = var free y :=
-  by simp [subst, h]
+@[simp] theorem subst_var_free_eq (h : x = y) : subst x tx (var free y) = tx :=
+by simp [subst, h]
 
-@[simp]
-theorem subst_arr {t₁ t₂ : typ V} : subst x t (arr t₁ t₂) = arr (subst x t t₁) (subst x t t₂) :=
-  rfl
+@[simp] theorem subst_var_free_ne (h : x ≠ y) : subst x tx (var free y) = var free y :=
+by simp [subst, h]
 
-@[simp]
-theorem subst_list_nil_left : subst_list [] ts t = t :=
-  rfl
-
-@[simp]
-theorem subst_list_nil_right : subst_list xs [] t = t :=
-  by cases xs; refl
-
-@[simp]
-theorem subst_list_cons_cons : subst_list (x :: xs) (tx :: ts) t = subst_list xs ts (subst x tx t) :=
-  rfl
+@[simp] theorem subst_arr : subst x tx (arr t₁ t₂) = arr (subst x tx t₁) (subst x tx t₂) :=
+rfl
 
 -- Substitution with a fresh name is the identity
-@[simp]
-theorem subst_fresh (h : x ∉ fv t) : subst x tx t = t :=
-  by induction t with o; try {cases o}; try {simp at h}; try {cases h}; simp *
+@[simp] theorem subst_fresh (h : x ∉ fv t) : subst x tx t = t :=
+by induction t with o; try {cases o}; try {simp at h}; try {cases h}; simp *
 
 -- Mapping substitution over a list with a fresh name is the identity
-@[simp]
-theorem subst_fresh_list (h : x ∉ fv_list ts) : list.map (subst x t) ts = ts :=
-  begin
-/-
-    induction ts with _ _ ih; simp [decidable.not_or_iff_and_not],
-    exact λ h₁ h₂, ⟨subst_fresh h₁, ih h₂⟩
--/
-    induction ts; try {simp at h}; try {cases h}; simp *
-  end
+@[simp] theorem subst_fresh_list (h : x ∉ fv_list ts) : map (subst x t) ts = ts :=
+by induction ts; try {simp at h}; try {cases h}; simp *
 
-@[simp]
-theorem subst_fresh_var_free (h : x ∉ xs)
-: list.map (subst x t) (list.map (var free) xs) = list.map (var free) xs :=
-  begin
-    apply subst_fresh_list,
-    induction xs with _ _ ih; simp,
-    exact ⟨list.ne_of_not_mem_cons h, ih (list.not_mem_of_not_mem_cons h)⟩
-  end
+@[simp] theorem subst_fresh_var_free (h : x ∉ xs) :
+  map (subst x tx) (map (var free) xs) = map (var free) xs :=
+begin
+  apply subst_fresh_list,
+  induction xs with _ _ ih; simp,
+  exact ⟨ne_of_not_mem_cons h, ih (not_mem_of_not_mem_cons h)⟩
+end
 
-@[simp]
-theorem subst_list_fresh (F : ∀ x ∈ xs, x ∉ fv t) : subst_list xs ts t = t :=
-  begin
-    induction xs generalizing ts t,
-    case list.nil { simp },
-    case list.cons : _ _ ih { simp at F, cases ts; [simp, {simp [F.1, ih F.2]}] }
-  end
+/- subst_list -/
+
+/-- Substitute a list of free variables for a list of types in a type -/
+def subst_list : list (tagged V) → list (typ V) → typ V → typ V
+| (x :: xs) (tx :: txs) t := subst_list xs txs (subst x tx t)
+| _         _           t := t
+
+@[simp] theorem subst_list_nil_left : subst_list [] txs t = t :=
+rfl
+
+@[simp] theorem subst_list_nil_right : subst_list xs [] t = t :=
+by cases xs; refl
+
+@[simp] theorem subst_list_cons_cons :
+  subst_list (x :: xs) (tx :: txs) t = subst_list xs txs (subst x tx t) :=
+rfl
+
+@[simp] theorem subst_list_fresh (F : ∀ x ∈ xs, x ∉ fv t) : subst_list xs txs t = t :=
+begin
+  induction xs generalizing txs t,
+  case list.nil { simp },
+  case list.cons : _ _ ih { simp at F, cases txs; [simp, {simp [F.1, ih F.2]}] }
+end
 
 -- Substitution distributes over open
-theorem subst_open (l₂ : lc t₂)
-: subst x t₂ (open_typs ts t₁) = open_typs (list.map (subst x t₂) ts) (subst x t₂ t₁) :=
-  begin
-    induction t₁,
-    case typ.var : o y {
-      cases o,
-      case occurs.bound { simp [list.nth_of_map] },
-      case occurs.free  { by_cases x = y; simp * }
-    },
-    case typ.arr { simp * }
-  end
+theorem subst_open_typs (lx : lc tx) :
+  subst x tx (open_typs ts t) = open_typs (map (subst x tx) ts) (subst x tx t) :=
+begin
+  induction t,
+  case typ.var : o y {
+    cases o,
+    case occurs.bound { simp [nth_of_map] },
+    case occurs.free  { by_cases x = y; simp * } },
+  case typ.arr { simp * }
+end
 
 -- Substitution and open_vars for distinct names commute
-theorem subst_open_vars (h : x ∉ xs) (l₂ : lc t₂)
-: open_vars xs (subst x t₂ t₁) = subst x t₂ (open_vars xs t₁) :=
-  by simp [open_vars, h, subst_open l₂]
+theorem subst_open_vars (h : x ∉ xs) (lx : lc tx) :
+  open_vars xs (subst x tx t) = subst x tx (open_vars xs t) :=
+by simp [open_vars, h, subst_open_typs lx]
 
 theorem subst_list_intro_aux
-(ts₂ : list (typ V))
-(d : xs.nodup)
-(ln_eq : xs.length = ts₁.length)
-(F : ∀ x ∈ xs, x ∉ fv t ∪ fv_list ts₁ ∪ fv_list ts₂)
-(l₁ : ∀ t ∈ ts₁, lc t)
-(l₂ : ∀ t ∈ ts₂, lc t)
-: open_typs (ts₂ ++ ts₁) t = subst_list xs ts₁ (open_typs (ts₂ ++ list.map (var free) xs) t) :=
-  begin
-    induction xs generalizing ts₁ ts₂ d,
-    case list.nil {
-      have : ts₁ = [] := list.length_eq_zero.mp (by simp at ln_eq; simp [ln_eq]),
-      simp [this]
-    },
-    case list.cons : hd tl ih {
-      cases ts₁; simp at ln_eq,
-      case list.nil { cases ln_eq },
-      case list.cons : hd₁ tl₁ {
-        simp at l₁,
-        have lhd₁ : lc hd₁ := l₁.1,
-        have ltl₁ : ∀ t ∈ tl₁, lc t := l₁.2,
-        clear l₁,
-        simp at F,
-        have hdFt   : hd ∉ fv t := F.1,
-        have hdFhd₁ : hd ∉ fv hd₁ := F.2.1,
-        have hdFts₂ : hd ∉ fv_list ts₂ := F.2.2.1,
-        have hdFts₂hd₁ : hd ∉ fv_list (ts₂ ++ [hd₁]),
-          by simp [hdFhd₁, hdFts₂],
-        have tlF    : ∀ x ∈ tl, x ∉ fv t ∪ fv_list tl₁ ∪ fv_list (ts₂ ++ [hd₁]) :=
-          λ x h, let H := F.2.2.2.2 x h in by simp [H.1, H.2.1, H.2.2.1, H.2.2.2],
-        clear hdFhd₁ F,
-        have lts₂hd₁ : ∀ t ∈ ts₂ ++ [hd₁], lc t :=
-          λ t h, by simp at h; cases h; simp [h, l₂ t, lhd₁],
-        simp at d,
-        have ih : open_typs (ts₂ ++ [hd₁] ++ tl₁) t =
-        subst_list tl tl₁ (open_typs (ts₂ ++ [hd₁] ++ list.map (var free) tl) t) :=
-          ih _ d.2 ln_eq tlF ltl₁ lts₂hd₁,
-        rw [list.append_cons_left, ih, ←list.append_cons_left],
-        simp [subst_open lhd₁, subst_fresh hdFt, subst_fresh_list hdFts₂, subst_fresh_var_free d.1]
-      },
-    }
-  end
+  (ts : list (typ V))
+  (d : xs.nodup)
+  (ln_eq : xs.length = txs.length)
+  (F : ∀ x ∈ xs, x ∉ fv t ∪ fv_list txs ∪ fv_list ts)
+  (ltxs : ∀ t ∈ txs, lc t)
+  (l₂ : ∀ t ∈ ts, lc t) :
+  open_typs (ts ++ txs) t = subst_list xs txs (open_typs (ts ++ map (var free) xs) t) :=
+begin
+  induction xs generalizing txs ts d,
+  case list.nil {
+    have : txs = [] := length_eq_zero.mp (by simp at ln_eq; simp [ln_eq]),
+    simp [this] },
+  case list.cons : hd tl ih {
+    cases txs; simp at ln_eq,
+    case list.nil { cases ln_eq },
+    case list.cons : hdxs tlxs {
+      simp at ltxs,
+      have lhdxs : lc hdxs := ltxs.1,
+      have ltlxs : ∀ t ∈ tlxs, lc t := ltxs.2,
+      simp at F,
+      have hdFt    : hd ∉ fv t := F.1,
+      have hdFhdxs : hd ∉ fv hdxs := F.2.1,
+      have hdFts   : hd ∉ fv_list ts := F.2.2.1,
+      have tlF     : ∀ x ∈ tl, x ∉ fv t ∪ fv_list tlxs ∪ fv_list (ts ++ [hdxs]) :=
+        λ x h, let H := F.2.2.2.2 x h in by simp [H.1, H.2.1, H.2.2.1, H.2.2.2],
+      have lts_hdxs : ∀ t ∈ ts ++ [hdxs], lc t :=
+        λ t h, by simp at h; cases h; simp [h, l₂ t, lhdxs],
+      simp at d,
+      have ih : open_typs (ts ++ [hdxs] ++ tlxs) t =
+      subst_list tl tlxs (open_typs (ts ++ [hdxs] ++ map (var free) tl) t) :=
+        ih _ d.2 ln_eq tlF ltlxs lts_hdxs,
+      rw [append_cons_left, ih, ←append_cons_left],
+      simp [subst_open_typs lhdxs, subst_fresh hdFt, subst_fresh_list hdFts, subst_fresh_var_free d.1] } }
+end
 
 -- Opening up a type `t` with `ts` is the same as opening up `t` with fresh
 -- names `xs` and then substituting `xs` for `ts`.
 theorem subst_list_intro
-(d : xs.nodup)
-(ln_eq : xs.length = ts.length)
-(F : ∀ x ∈ xs, x ∉ fv t ∪ fv_list ts)
-(l : ∀ t ∈ ts, lc t)
-: open_typs ts t = subst_list xs ts (open_vars xs t) :=
-  subst_list_intro_aux [] d ln_eq (λ x, by simpa using F x) l (by simp)
+  (d : xs.nodup)
+  (ln_eq : xs.length = ts.length)
+  (F : ∀ x ∈ xs, x ∉ fv t ∪ fv_list ts)
+  (l : ∀ t ∈ ts, lc t) :
+  open_typs ts t = subst_list xs ts (open_vars xs t) :=
+subst_list_intro_aux [] d ln_eq (λ x, by simpa using F x) l (by simp)
 
 -- A type substituted with another type is locally-closed if all type arguments
 -- are locally-closed.
-theorem subst_lc (l₂ : lc t₂) (l₁ : lc t₁) : lc (subst x t₂ t₁) :=
-  begin
-    induction l₁,
-    case lc.var : y { by_cases h : x = y; simp [h, l₂] },
-    case lc.arr { simp * }
-  end
+theorem subst_lc (lx : lc tx) (l : lc t) : lc (subst x tx t) :=
+begin
+  induction l,
+  case lc.var : y { by_cases h : x = y; simp [h, lx] },
+  case lc.arr { simp * }
+end
 
 -- A type substituted with a list of types is locally-closed if all type
 -- arguments are locally-closed.
 theorem subst_list_lc
-(ln_eq : xs.length = ts.length)
-(lts : ∀ t ∈ ts, lc t)
-(lt : lc t)
-: lc (subst_list xs ts t) :=
-  begin
-    induction xs generalizing ts t,
+  (ln_eq : xs.length = txs.length)
+  (ltxs : ∀ tx ∈ txs, lc tx)
+  (lt : lc t) :
+  lc (subst_list xs txs t) :=
+begin
+  induction xs generalizing txs t,
+  case list.nil { simp [lt] },
+  case list.cons : _ _ ih {
+    cases txs,
     case list.nil { simp [lt] },
-    case list.cons : _ _ ih {
-      cases ts,
-      case list.nil { simp [lt] },
-      case list.cons {
-        simp at ln_eq,
-        simp at lts,
-        simp [ih ln_eq lts.2 (subst_lc lts.1 lt)]
-      }
-    }
-  end
+    case list.cons {
+      simp at ln_eq,
+      simp at ltxs,
+      simp [ih ln_eq ltxs.2 (subst_lc ltxs.1 lt)] } }
+end
 
 -- Mapping substitution over a list of types is locally-closed if all type
 -- arguments are locally-closed.
-theorem map_subst_lc (lt : lc t) (lts : ∀ t ∈ ts, lc t)
-: ∀ t ∈ list.map (subst x t) ts, lc t :=
-  begin
-    induction ts,
-    case list.nil { simp },
-    case list.cons : _ _ ih {
-      simp at lts,
-      exact list.forall_mem_cons.mpr ⟨subst_lc lt lts.1, ih lts.2⟩
-    }
-  end
+theorem map_subst_lc (lt : lc t) (lts : ∀ t ∈ ts, lc t) :
+  ∀ t ∈ map (subst x t) ts, lc t :=
+begin
+  induction ts,
+  case list.nil { simp },
+  case list.cons : _ _ ih {
+    simp at lts,
+    exact forall_mem_cons.mpr ⟨subst_lc lt lts.1, ih lts.2⟩ }
+end
 
 end /- namespace -/ typ --------------------------------------------------------
 end /- namespace -/ tts --------------------------------------------------------
